Rsa encryption refactor (#114)
* Refactor RSAEncryption to remove unused methods, remove duplicate code

* Add method to get Modulus from public key to CS

* Remove additional RSA prefix from names within RSAEncryption

* Refactor to remove need to specify extern for RSA Encrypt/Decrypt

* Bug fix, now reading private key correctly, tests pass

* Update wording to make the RSAEncryption math clearer

* Add preconditions to RSAEncryption externs

* Add Def to module names for AES and RSA to avoid future issues when using externs

* Add precondition for public/private key length > 0 when it exists, refactor RSAEncryptionDef subclass externs

* Switch to RsaBlindedEnginer, change wording around RSA strength

* Wrap Private/Public keys in class for additional verification and type safety

* Verify all RSA padding modes via RawRSAKeyring tests

* Formatting fixes, made unnecessary function methods just functions

* Further ensure that the strenght and padding are not changed after initial pem generation

test/SDK/Keyring/RawRSAKeyring.dfy
@@ -8,45 +8,77 @@ include "../../../src/Util/UTF8.dfy"
 module TestRSAKeyring {
   import opened StandardLibrary
   import opened UInt = StandardLibrary.UInt
-  import RSAEncryption
+  import RSA = RSAEncryption
   import RawRSAKeyringDef
   import AlgorithmSuite
   import UTF8
 
   const name := UTF8.Encode("test Name").value;
   const namespace := UTF8.Encode("test Namespace").value;
+  const allPaddingModes := {RSA.PKCS1, RSA.OAEP_SHA1, RSA.OAEP_SHA256, RSA.OAEP_SHA384, RSA.OAEP_SHA512}
 
   method {:test} TestOnEncryptOnDecryptGenerateDataKey() returns (r: Result<()>)
   {
-    var ek, dk := RSAEncryption.RSA.RSAKeygen(2048, RSAEncryption.PKCS1);
-    var rawRSAKeyring := new RawRSAKeyringDef.RawRSAKeyring(name, namespace, RSAEncryption.RSAPaddingMode.PKCS1, Some(ek), Some(dk));
-    
-    var keyA, valA := UTF8.Encode("keyA").value, UTF8.Encode("valA").value;
-    var encryptionContext := [(keyA, valA)];
-    var onEncryptResult :- rawRSAKeyring.OnEncrypt(AlgorithmSuite.AES_256_GCM_IV12_TAG16_HKDF_SHA384_ECDSA_P384, encryptionContext, None);
-    var _ :- Require(onEncryptResult.Some? && |onEncryptResult.get.encryptedDataKeys| == 1);
+    var remainingPaddingModes := allPaddingModes;
+    var allResults: seq<Result<()>> := [];
+    while remainingPaddingModes != {}
+      invariant |remainingPaddingModes| + |allResults| == |allPaddingModes|
+      decreases remainingPaddingModes
+    {
+      var paddingMode :| paddingMode in remainingPaddingModes;
+      remainingPaddingModes := remainingPaddingModes - {paddingMode};
+      // Verify key generation for a given padding mode
+      var publicKey, privateKey := RSA.GenerateKeyPair(2048, paddingMode);
+      var rawRSAKeyring := new RawRSAKeyringDef.RawRSAKeyring(name, namespace, paddingMode, Some(publicKey), Some(privateKey));
 
-    var pdk := onEncryptResult.get.plaintextDataKey;
-    var edk := onEncryptResult.get.encryptedDataKeys[0];
+      // Verify encoding
+      var keyA, valA := UTF8.Encode("keyA").value, UTF8.Encode("valA").value;
+      var encryptionContext := [(keyA, valA)];
+      var onEncryptResult :- rawRSAKeyring.OnEncrypt(AlgorithmSuite.AES_256_GCM_IV12_TAG16_HKDF_SHA384_ECDSA_P384, encryptionContext, None);
+      var _ :- Require(onEncryptResult.Some? &&
+        |onEncryptResult.get.encryptedDataKeys| == 1 &&
+        |onEncryptResult.get.keyringTrace| == 2);
+      var plaintextDataKey := onEncryptResult.get.plaintextDataKey;
+      var encryptedDataKey := onEncryptResult.get.encryptedDataKeys[0];
 
-    var res :- rawRSAKeyring.OnDecrypt(AlgorithmSuite.AES_256_GCM_IV12_TAG16_HKDF_SHA384_ECDSA_P384, encryptionContext, [edk]);
-    r := Require(res.Some? && res.get.plaintextDataKey == pdk);
+      // Verify decoding
+      var res :- rawRSAKeyring.OnDecrypt(AlgorithmSuite.AES_256_GCM_IV12_TAG16_HKDF_SHA384_ECDSA_P384, encryptionContext, [encryptedDataKey]);
+      var newResultVerification := Require(res.Some? && res.get.plaintextDataKey == plaintextDataKey);
+      allResults := allResults + [newResultVerification];
+    }
+    r := Require(|allResults| == |allPaddingModes| && forall result :: result in allResults ==> result.Success?);
   }
 
   method {:test} TestOnEncryptOnDecryptSuppliedDataKey() returns (r: Result<()>)
   {
-    var ek, dk := RSAEncryption.RSA.RSAKeygen(2048, RSAEncryption.PKCS1);
-    var rawRSAKeyring := new RawRSAKeyringDef.RawRSAKeyring(name, namespace, RSAEncryption.RSAPaddingMode.PKCS1, Some(ek), Some(dk));
-    
-    var keyA, valA := UTF8.Encode("keyA").value, UTF8.Encode("valA").value;
-    var encryptionContext := [(keyA, valA)];
-    var pdk := seq(32, i => 0);
-    var onEncryptResult :- rawRSAKeyring.OnEncrypt(AlgorithmSuite.AES_256_GCM_IV12_TAG16_HKDF_SHA384_ECDSA_P384, encryptionContext, Some(pdk));
-    var _ :- Require(onEncryptResult.Some? && |onEncryptResult.get.encryptedDataKeys| == 1);
-    
-    var edk := onEncryptResult.get.encryptedDataKeys[0];
+    var remainingPaddingModes := allPaddingModes;
+    var allResults: seq<Result<()>> := [];
+    while remainingPaddingModes != {}
+      invariant |remainingPaddingModes| + |allResults| == |allPaddingModes|
+      decreases remainingPaddingModes
+    {
+      var paddingMode :| paddingMode in remainingPaddingModes;
+      remainingPaddingModes := remainingPaddingModes - {paddingMode};
+      // Verify key generation for a given padding mode
+      var publicKey, privateKey := RSA.GenerateKeyPair(2048, paddingMode);
+      var rawRSAKeyring := new RawRSAKeyringDef.RawRSAKeyring(name, namespace, paddingMode, Some(publicKey), Some(privateKey));
 
-    var res :- rawRSAKeyring.OnDecrypt(AlgorithmSuite.AES_256_GCM_IV12_TAG16_HKDF_SHA384_ECDSA_P384, encryptionContext, [edk]);
-    r := Require(res.Some? && res.get.plaintextDataKey == pdk);
+      // Verify encoding
+      var keyA, valA := UTF8.Encode("keyA").value, UTF8.Encode("valA").value;
+      var encryptionContext := [(keyA, valA)];
+      var plaintextDataKey := seq(32, i => 0);
+      var onEncryptResult :- rawRSAKeyring.OnEncrypt(AlgorithmSuite.AES_256_GCM_IV12_TAG16_HKDF_SHA384_ECDSA_P384, encryptionContext, Some(plaintextDataKey));
+      var _ :- Require(onEncryptResult.Some? &&
+        |onEncryptResult.get.encryptedDataKeys| == 1 &&
+        onEncryptResult.get.plaintextDataKey == plaintextDataKey &&
+        |onEncryptResult.get.keyringTrace| == 1);
+      var encryptedDataKey := onEncryptResult.get.encryptedDataKeys[0];
+
+      // Verify decoding
+      var res :- rawRSAKeyring.OnDecrypt(AlgorithmSuite.AES_256_GCM_IV12_TAG16_HKDF_SHA384_ECDSA_P384, encryptionContext, [encryptedDataKey]);
+      var newResultVerification := Require(res.Some? && res.get.plaintextDataKey == plaintextDataKey);
+      allResults := allResults + [newResultVerification];
+    }
+    r := Require(|allResults| == |allPaddingModes| && forall result :: result in allResults ==> result.Success?);
   }
 }
